Foundation/Modal/Kripke/Hilbert/K5.lean
@@ -6,7 +6,7 @@ open Kripke
 open Geachean
 
 abbrev Kripke.EuclideanFrameClass : FrameClass := { F | Euclidean F }
-abbrev Kripke.EuclideanFiniteFrameClass : FiniteFrameClass := { F | Euclidean F.Rel }
+-- abbrev Kripke.EuclideanFiniteFrameClass : FiniteFrameClass := { F | Euclidean F.Rel }
 
 namespace Hilbert.K5
 
@@ -20,11 +20,9 @@ instance Kripke.consistent : Entailment.Consistent (Hilbert.K5) := by
   convert Hilbert.Geach.Kripke.Consistent (G := {⟨1, 1, 0, 1⟩});
   exact eq_Geach;
 
-instance Kripke.complete : Complete (Hilbert.K5) (Kripke.EuclideanFrameClass) := by
-  convert Hilbert.Geach.Kripke.Complete (G := {⟨1, 1, 0, 1⟩});
-  . exact eq_Geach;
-  . unfold EuclideanFrameClass MultiGeacheanConfluentFrameClass MultiGeachean;
-    simp [Geachean.euclidean_def];
+instance Kripke.canonical : Canonical (Hilbert.K5) (Kripke.EuclideanFrameClass) := ⟨Canonical.euclidean⟩
+
+instance Kripke.complete : Complete (Hilbert.K5) (Kripke.EuclideanFrameClass) := inferInstance
 
 end Hilbert.K5
 
