Foundation/Modal/Kripke/Hilbert/S4Dot2.lean
@@ -19,11 +19,9 @@ instance Kripke.consistent : Entailment.Consistent (Hilbert.S4Dot2) := by
   convert Hilbert.Geach.Kripke.Consistent (G := {⟨0, 0, 1, 0⟩, ⟨0, 2, 1, 0⟩, ⟨1, 1, 1, 1⟩});
   exact eq_Geach;
 
-instance Kripke.complete : Complete (Hilbert.S4Dot2) (ReflexiveTransitiveConfluentFrameClass) := by
-  convert Hilbert.Geach.Kripke.Complete (G := {⟨0, 0, 1, 0⟩, ⟨0, 2, 1, 0⟩, ⟨1, 1, 1, 1⟩});
-  . exact eq_Geach;
-  . unfold ReflexiveTransitiveConfluentFrameClass MultiGeacheanConfluentFrameClass MultiGeachean;
-    simp [Geachean.reflexive_def, Geachean.transitive_def, Geachean.confluent_def];
+instance Kripke.canonical : Canonical (Hilbert.S4Dot2) (ReflexiveTransitiveConfluentFrameClass) := ⟨⟨Canonical.reflexive, Canonical.transitive, Canonical.confluent⟩⟩
+
+instance Kripke.complete : Complete (Hilbert.S4Dot2) (ReflexiveTransitiveConfluentFrameClass) := inferInstance
 
 end Hilbert.S4Dot2
 
