Foundation/Modal/Tableau.lean
@@ -1,0 +1,748 @@
+import Foundation.Modal.Formula
+import Foundation.Modal.Entailment.K
+
+namespace LO.Modal
+
+open Entailment
+variable {α : Type*}
+variable {S} [Entailment (Formula α) S]
+variable {𝓢 : S}
+
+
+def Tableau (α : Type u) := Set (Formula α) × Set (Formula α)
+
+namespace Tableau
+
+variable {t : Tableau α} {φ ψ : Formula α}
+
+protected def Consistent (𝓢 : S) (t : Tableau α) := ∀ {Γ Δ : List (Formula α)}, (∀ φ ∈ Γ, φ ∈ t.1) → (∀ φ ∈ Δ, φ ∈ t.2) → 𝓢 ⊬ ⋀Γ ➝ ⋁Δ
+
+protected abbrev Inconsistent (𝓢 : S) (t : Tableau α) := ¬t.Consistent 𝓢
+
+protected structure Saturated (t : Tableau α) : Prop where
+  imply₁ {φ ψ} : φ ➝ ψ ∈ t.1 → φ ∈ t.2 ∨ ψ ∈ t.1
+  imply₂ {φ ψ} : φ ➝ ψ ∈ t.2 → φ ∈ t.1 ∧ ψ ∈ t.2
+
+protected structure Disjoint (t : Tableau α) : Prop where
+  union : Disjoint t.1 t.2
+  no_bot : ⊥ ∉ t.1
+
+protected def Maximal (t : Tableau α) := ∀ {φ}, φ ∈ t.1 ∨ φ ∈ t.2
+
+instance : HasSubset (Tableau α) := ⟨λ t₁ t₂ => t₁.1 ⊆ t₂.1 ∧ t₁.2 ⊆ t₂.2⟩
+@[simp] lemma subset_def {t₁ t₂ : Tableau α} : t₁ ⊆ t₂ ↔ t₁.1 ⊆ t₂.1 ∧ t₁.2 ⊆ t₂.2 := by rfl
+
+
+section
+
+variable [Entailment.K 𝓢]
+
+lemma equality_def {t₁ t₂ : Tableau α} : t₁ = t₂ ↔ t₁.1 = t₂.1 ∧ t₁.2 = t₂.2 := by
+  constructor;
+  . intro h; cases h; simp;
+  . rintro ⟨h₁, h₂⟩; cases t₁; cases t₂; simp_all;
+
+lemma disjoint_of_consistent (hCon : t.Consistent 𝓢) : t.Disjoint := by
+  constructor;
+  . by_contra hC;
+    obtain ⟨T, hT₁, hT₂, hT⟩ := by simpa [Disjoint] using hC;
+    obtain ⟨φ, hφ⟩ := Set.nonempty_def.mp $ Set.nonempty_iff_ne_empty.mpr hT;
+    unfold Tableau.Consistent at hCon;
+    have : 𝓢 ⊬ ⋀[φ] ➝ ⋁[φ] := hCon
+      (by simp_all; apply hT₁; assumption)
+      (by simp_all; apply hT₂; assumption);
+    have : 𝓢 ⊢! ⋀[φ] ➝ ⋁[φ] := by simp;
+    contradiction;
+  . by_contra hC;
+    exact hCon (Γ := [⊥]) (Δ := []) (by simpa) (by simp) $ by simp;
+
+lemma mem₂_of_not_mem₁ (hMax : t.Maximal) : φ ∉ t.1 → φ ∈ t.2 := by
+  intro h;
+  cases hMax with
+  | inl h' => contradiction;
+  | inr _ => assumption;
+
+lemma mem₁_of_not_mem₂ (hMax : t.Maximal) : φ ∉ t.2 → φ ∈ t.1 := by
+  intro h;
+  cases hMax with
+  | inl _ => assumption;
+  | inr h' => contradiction;
+
+lemma iff_not_mem₁_mem₂ (hCon : t.Consistent 𝓢) (hMax : t.Maximal) : φ ∉ t.1 ↔ φ ∈ t.2 := by
+  constructor;
+  . apply mem₂_of_not_mem₁ hMax;
+  . apply Set.disjoint_right.mp $ disjoint_of_consistent hCon |>.1;
+
+lemma iff_not_mem₂_mem₁ (hCon : t.Consistent 𝓢) (hMax : t.Maximal) : φ ∉ t.2 ↔ φ ∈ t.1 := by
+  constructor;
+  . apply mem₁_of_not_mem₂ hMax;
+  . apply Set.disjoint_left.mp $ disjoint_of_consistent hCon |>.1;
+
+lemma maximal_duality
+  {t₁ t₂ : Tableau α}
+  (hCon₁ : t₁.Consistent 𝓢) (hCon₂ : t₂.Consistent 𝓢)
+  (hMax₁ : t₁.Maximal) (hMax₂ : t₂.Maximal)
+  : t₁.1 = t₂.1 ↔ t₁.2 = t₂.2 := by
+  constructor;
+  . intro h;
+    apply Set.eq_of_subset_of_subset;
+    . intro φ hp;
+      apply iff_not_mem₁_mem₂ hCon₂ hMax₂ |>.mp; rw [←h];
+      apply iff_not_mem₁_mem₂ hCon₁ hMax₁ |>.mpr hp;
+    . intro φ hp;
+      apply iff_not_mem₁_mem₂ hCon₁ hMax₁ |>.mp; rw [h];
+      apply iff_not_mem₁_mem₂ hCon₂ hMax₂ |>.mpr hp;
+  . intro h;
+    apply Set.eq_of_subset_of_subset;
+    . intro φ hp;
+      apply iff_not_mem₂_mem₁ hCon₂ hMax₂ |>.mp; rw [←h];
+      apply iff_not_mem₂_mem₁ hCon₁ hMax₁ |>.mpr hp;
+    . intro φ hp;
+      apply iff_not_mem₂_mem₁ hCon₁ hMax₁ |>.mp; rw [h];
+      apply iff_not_mem₂_mem₁ hCon₂ hMax₂ |>.mpr hp;
+
+variable [DecidableEq α]
+
+lemma iff_consistent_insert₁
+  : Tableau.Consistent 𝓢 ((insert φ T), U) ↔ ∀ {Γ Δ : List (Formula α)}, (∀ φ ∈ Γ, φ ∈ T) → (∀ φ ∈ Δ, φ ∈ U) → 𝓢 ⊬ φ ⋏ ⋀Γ ➝ ⋁Δ := by
+  constructor;
+  . intro h Γ Δ hΓ hΔ;
+    by_contra hC;
+    have : 𝓢 ⊬ ⋀(φ :: Γ) ➝ ⋁Δ := h (by simp; intro ψ hψ; right; exact hΓ ψ hψ;) hΔ;
+    have : 𝓢 ⊢! ⋀(φ :: Γ) ➝ ⋁Δ := iff_imply_left_cons_conj'!.mpr hC;
+    contradiction;
+  . intro h Γ Δ hΓ hΔ;
+    simp_all only [Set.mem_insert_iff];
+    have : 𝓢 ⊬ φ ⋏ ⋀(Γ.remove φ) ➝ ⋁Δ := h (by
+      intro ψ hq;
+      have := by simpa using hΓ ψ $ List.mem_of_mem_remove hq;
+      cases this with
+      | inl h => simpa [h] using List.mem_remove_iff.mp hq;
+      | inr h => assumption;
+    ) hΔ;
+    by_contra hC;
+    have : 𝓢 ⊢! φ ⋏ ⋀(Γ.remove φ) ➝ ⋁Δ := imp_trans''! and_comm! $ imply_left_remove_conj! (φ := φ) hC;
+    contradiction;
+
+lemma iff_inconsistent_insert₁ : Tableau.Inconsistent 𝓢 ((insert φ T), U) ↔ ∃ Γ Δ : List (Formula α), (∀ φ ∈ Γ, φ ∈ T) ∧ (∀ φ ∈ Δ, φ ∈ U) ∧ 𝓢 ⊢! φ ⋏ ⋀Γ ➝ ⋁Δ := by
+  unfold Tableau.Inconsistent;
+  constructor;
+  . contrapose; push_neg; apply iff_consistent_insert₁.mpr;
+  . contrapose; push_neg; apply iff_consistent_insert₁.mp;
+
+lemma iff_consistent_insert₂ : Tableau.Consistent 𝓢 (T, (insert φ U)) ↔ ∀ {Γ Δ : List (Formula α)}, (∀ φ ∈ Γ, φ ∈ T) → (∀ φ ∈ Δ, φ ∈ U) → 𝓢 ⊬ ⋀Γ ➝ φ ⋎ ⋁Δ := by
+  constructor;
+  . intro h Γ Δ hΓ hΔ;
+    by_contra hC;
+    have : 𝓢 ⊬ ⋀Γ ➝ ⋁(φ :: Δ) := h hΓ (by simp; intro ψ hq; right; exact hΔ ψ hq);
+    have : 𝓢 ⊢! ⋀Γ ➝ ⋁(φ :: Δ) := implyRight_cons_disj!.mpr hC;
+    contradiction;
+  . intro h Γ Δ hΓ hΔ;
+    simp_all;
+    have : 𝓢 ⊬ ⋀Γ ➝ φ ⋎ ⋁(Δ.remove φ) := h hΓ (by
+      intro ψ hq;
+      have := by simpa using hΔ ψ $ List.mem_of_mem_remove hq;
+      cases this with
+      | inl h => simpa [h] using List.mem_remove_iff.mp hq;
+      | inr h => assumption;
+    );
+    by_contra hC;
+    have : 𝓢 ⊢! ⋀Γ ➝ φ ⋎ ⋁(Δ.remove φ) := imp_trans''! hC $ forthback_disj_remove;
+    contradiction;
+
+lemma iff_not_consistent_insert₂ : Tableau.Inconsistent 𝓢 (T, (insert φ U)) ↔ ∃ Γ Δ : List (Formula α), (∀ φ ∈ Γ, φ ∈ T) ∧ (∀ φ ∈ Δ, φ ∈ U) ∧ 𝓢 ⊢! ⋀Γ ➝ φ ⋎ ⋁Δ := by
+  unfold Tableau.Inconsistent;
+  constructor;
+  . contrapose; push_neg; apply iff_consistent_insert₂.mpr;
+  . contrapose; push_neg; apply iff_consistent_insert₂.mp;
+
+lemma iff_consistent_empty_singleton₂ : Tableau.Consistent 𝓢 (∅, {φ}) ↔ 𝓢 ⊬ φ := by
+  convert iff_consistent_insert₂ (𝓢 := 𝓢) (T := ∅) (U := ∅) (φ := φ);
+  . simp;
+  . constructor;
+    . contrapose;
+      push_neg;
+      rintro ⟨Γ, Δ, hΓ, hΔ, h⟩;
+      have : Γ = [] := List.eq_nil_iff_forall_not_mem.mpr hΓ;
+      have : Δ = [] := List.eq_nil_iff_forall_not_mem.mpr hΔ;
+      subst Γ Δ;
+      simpa using or_cases! imp_id! efq! ((by simpa using h) ⨀ verum!);
+    . contrapose;
+      push_neg;
+      intro h;
+      use [], [];
+      refine ⟨by tauto, by tauto, ?_⟩;
+      simp only [List.conj₂_nil, List.disj₂_nil, not_not];
+      apply imply₁'!;
+      apply or₁'! (by simpa using h);
+
+lemma iff_inconsistent_singleton₂ : Tableau.Inconsistent 𝓢 (∅, {φ}) ↔ 𝓢 ⊢! φ := by
+  convert iff_consistent_empty_singleton₂ (𝓢 := 𝓢) (φ := φ) |>.not;
+  tauto;
+
+lemma either_expand_consistent_of_consistent (hCon : t.Consistent 𝓢) (φ : Formula α) : Tableau.Consistent 𝓢 ((insert φ t.1), t.2) ∨ Tableau.Consistent 𝓢 (t.1, (insert φ t.2)) := by
+  by_contra hC;
+  push_neg at hC;
+  have ⟨hC₁, hC₂⟩ := hC;
+
+  obtain ⟨Γ₁, Δ₁, hΓ₁, hΔ₁, h₁⟩ := iff_inconsistent_insert₁.mp hC₁;
+  obtain ⟨Γ₂, Δ₂, hΓ₂, hΔ₂, h₂⟩ := iff_not_consistent_insert₂.mp hC₂;
+
+  replace h₁ := imply_left_and_comm'! h₁;
+
+  have : 𝓢 ⊢! ⋀(Γ₁ ++ Γ₂) ➝ ⋁(Δ₁ ++ Δ₂) := imp_trans''! (and₁'! iff_concat_conj!) $ imp_trans''! (cut! h₁ h₂) (and₂'! iff_concact_disj!);
+  have : 𝓢 ⊬ ⋀(Γ₁ ++ Γ₂) ➝ ⋁(Δ₁ ++ Δ₂) := hCon
+    (by simp; rintro ψ (hq₁ | hq₂); exact hΓ₁ ψ hq₁; exact hΓ₂ ψ hq₂)
+    (by simp; rintro ψ (hq₁ | hq₂); exact hΔ₁ ψ hq₁; exact hΔ₂ ψ hq₂);
+  contradiction;
+
+lemma consistent_empty [H_consis : Entailment.Consistent 𝓢] : Tableau.Consistent 𝓢 ⟨∅, ∅⟩ := by
+  intro Γ Δ hΓ hΔ;
+  replace hΓ : Γ = [] := List.eq_nil_iff_forall_not_mem.mpr hΓ;
+  replace hΔ : Δ = [] := List.eq_nil_iff_forall_not_mem.mpr hΔ;
+  subst hΓ hΔ;
+  by_contra hC;
+  simp only [List.conj₂_nil, List.disj₂_nil] at hC;
+  obtain ⟨ψ, hψ⟩ := H_consis.exists_unprovable;
+  have : 𝓢 ⊢! ψ := efq'! (hC ⨀ imp_id!);
+  contradiction;
+
+end
+
+
+section lindenbaum
+
+open Classical
+open Encodable
+
+variable {t : Tableau α}
+
+variable (𝓢 : S)
+
+def lindenbaum_next (φ : Formula α) (t : Tableau α) : Tableau α := if Tableau.Consistent 𝓢 (insert φ t.1, t.2) then (insert φ t.1, t.2) else (t.1, insert φ t.2)
+
+def lindenbaum_indexed [Encodable α] (t : Tableau α) : ℕ → Tableau α
+  | 0 => t
+  | i + 1 =>
+    match (decode i) with
+    | some φ => (lindenbaum_indexed t i).lindenbaum_next 𝓢 φ
+    | none => lindenbaum_indexed t i
+local notation:max t"[" i "]" => lindenbaum_indexed 𝓢 t i
+
+def lindenbaum_max [Encodable α] (t : Tableau α) : Tableau α := (⋃ i, t[i].1, ⋃ i, t[i].2)
+local notation:max t"∞" => lindenbaum_max 𝓢 t
+
+variable {𝓢}
+
+@[simp] lemma eq_lindenbaum_indexed_zero [Encodable α] {t : Tableau α} : t[0] = t := by simp [lindenbaum_indexed]
+
+lemma consistent_lindenbaum_next [Entailment.K 𝓢] (consistent : t.Consistent 𝓢) (φ : Formula α) : (t.lindenbaum_next 𝓢 φ).Consistent 𝓢 := by
+  unfold lindenbaum_next;
+  split;
+  . assumption;
+  . rcases (either_expand_consistent_of_consistent consistent φ) with (h | h);
+    . contradiction;
+    . assumption;
+
+variable [Encodable α]
+
+lemma consistent_lindenbaum_indexed_succ [Entailment.K 𝓢] {i : ℕ} : t[i].Consistent 𝓢 → t[i + 1].Consistent 𝓢 := by
+  simp only [lindenbaum_indexed];
+  split;
+  . intro h; apply consistent_lindenbaum_next h;
+  . tauto;
+
+lemma either_mem_lindenbaum_indexed (t) (φ : Formula α) : φ ∈ t[(encode φ) + 1].1 ∨ φ ∈ t[(encode φ) + 1].2 := by
+  simp only [lindenbaum_indexed, encodek, lindenbaum_next];
+  split <;> tauto;
+
+lemma consistent_lindenbaum_indexed [Entailment.K 𝓢] (consistent : t.Consistent 𝓢) (i : ℕ) : t[i].Consistent 𝓢 := by
+  induction i with
+  | zero => simpa;
+  | succ i ih => apply consistent_lindenbaum_indexed_succ; assumption;
+
+variable {m n : ℕ}
+
+lemma subset₁_lindenbaum_indexed_of_lt (h : m ≤ n) : t[m].1 ⊆ t[n].1 := by
+  induction h with
+  | refl => simp;
+  | step h ih =>
+    simp [lindenbaum_indexed, lindenbaum_next];
+    split;
+    . split <;> tauto;
+    . tauto;
+
+lemma subset₂_lindenbaum_indexed_of_lt (h : m ≤ n) : t[m].2 ⊆ t[n].2 := by
+  induction h with
+  | refl => simp;
+  | step h ih =>
+    simp [lindenbaum_indexed, lindenbaum_next];
+    split;
+    . split <;> tauto;
+    . tauto;
+
+lemma exists_consistent_saturated_tableau [Entailment.K 𝓢] (hCon : t.Consistent 𝓢) : ∃ u, t ⊆ u ∧ (u.Consistent 𝓢) ∧ (u.Maximal) := by
+  use t∞;
+  refine ⟨?subset, ?consistent, ?maximal⟩;
+  case subset => constructor <;> apply Set.subset_iUnion_of_subset 0 (by simp);
+  case maximal =>
+    intro φ;
+    rcases either_mem_lindenbaum_indexed (𝓢 := 𝓢) t φ with (h | h);
+    . left; simp only [lindenbaum_max, Set.mem_iUnion]; use (encode φ + 1);
+    . right; simp only [lindenbaum_max, Set.mem_iUnion];  use (encode φ + 1);
+  case consistent =>
+    intro Γ Δ hΓ hΔ;
+    simp_all only [lindenbaum_max, Set.mem_iUnion];
+    obtain ⟨m, hΓ⟩ : ∃ m, ∀ φ ∈ Γ, φ ∈ t[m].1 := by
+      induction Γ with
+      | nil => simp;
+      | cons φ Γ ih =>
+        simp_all only [List.mem_cons, or_true, implies_true, forall_const, forall_eq_or_imp];
+        obtain ⟨i, hi⟩ := hΓ.1;
+        obtain ⟨m, hm⟩ := ih;
+        use (i + m);
+        constructor;
+        . exact subset₁_lindenbaum_indexed_of_lt (by omega) hi;
+        . intro ψ hq;
+          exact subset₁_lindenbaum_indexed_of_lt (by omega) $ hm ψ hq;
+    obtain ⟨n, hΔ⟩ : ∃ n, ∀ φ ∈ Δ, φ ∈ t[n].2 := by
+      induction Δ with
+      | nil => simp;
+      | cons φ Δ ih =>
+        simp_all only [List.mem_cons, or_true, implies_true, forall_const, forall_eq_or_imp];
+        obtain ⟨i, hi⟩ := hΔ.1;
+        obtain ⟨n, hn⟩ := ih;
+        use (i + n);
+        constructor;
+        . exact subset₂_lindenbaum_indexed_of_lt (by omega) hi;
+        . intro ψ hq;
+          exact subset₂_lindenbaum_indexed_of_lt (by omega) $ hn ψ hq;
+    rcases (lt_trichotomy m n) with hm | hmn | hn;
+    . exact consistent_lindenbaum_indexed hCon n (by intro φ hp; exact subset₁_lindenbaum_indexed_of_lt hm.le $ hΓ φ hp) hΔ;
+    . subst hmn;
+      exact consistent_lindenbaum_indexed hCon m hΓ hΔ;
+    . exact consistent_lindenbaum_indexed hCon m hΓ (by intro φ hp; exact subset₂_lindenbaum_indexed_of_lt hn.le $ hΔ φ hp);
+
+protected alias lindenbaum := exists_consistent_saturated_tableau
+
+end lindenbaum
+
+end Tableau
+
+
+open Tableau
+
+def MaximalConsistentTableau (𝓢 : S) := {t : Tableau α // t.Maximal ∧ t.Consistent 𝓢}
+
+namespace MaximalConsistentTableau
+
+variable {t t₁ t₂  : MaximalConsistentTableau 𝓢} {φ ψ : Formula α}
+
+@[simp] lemma maximal (t : MaximalConsistentTableau 𝓢) : t.1.Maximal := t.2.1
+
+@[simp] lemma consistent (t : MaximalConsistentTableau 𝓢) : t.1.Consistent 𝓢 := t.2.2
+
+lemma lindenbaum {t₀ : Tableau α} [Entailment.K 𝓢] [Encodable α] (hCon : t₀.Consistent 𝓢) : ∃ (t : MaximalConsistentTableau 𝓢), t₀ ⊆ t.1 := by
+  obtain ⟨t, ht, hCon, hMax⟩ := Tableau.lindenbaum hCon;
+  exact ⟨⟨t, hMax, hCon⟩, ht⟩;
+
+instance [Entailment.Consistent 𝓢] [Entailment.K 𝓢] [DecidableEq α] [Encodable α] : Nonempty (MaximalConsistentTableau 𝓢) := ⟨lindenbaum consistent_empty |>.choose⟩
+
+variable {t t₁ t₂ : MaximalConsistentTableau 𝓢}
+
+variable [Entailment.K 𝓢]
+
+lemma disjoint : t.1.Disjoint := t.1.disjoint_of_consistent $ t.consistent
+
+lemma iff_not_mem₁_mem₂ : φ ∉ t.1.1 ↔ φ ∈ t.1.2 := Tableau.iff_not_mem₁_mem₂ t.consistent t.maximal
+
+lemma iff_not_mem₂_mem₁ : φ ∉ t.1.2 ↔ φ ∈ t.1.1 := Tableau.iff_not_mem₂_mem₁ t.consistent t.maximal
+
+lemma neither : ¬(φ ∈ t.1.1 ∧ φ ∈ t.1.2) := by
+  push_neg;
+  intro h;
+  exact iff_not_mem₂_mem₁.mpr h;
+
+lemma maximal_duality: t₁.1.1 = t₂.1.1 ↔ t₁.1.2 = t₂.1.2 :=
+  Tableau.maximal_duality t₁.consistent t₂.consistent t₁.maximal t₂.maximal
+
+lemma equality_of₁ (e₁ : t₁.1.1 = t₂.1.1) : t₁ = t₂ := by
+  have e := Tableau.equality_def.mpr ⟨e₁, (maximal_duality.mp e₁)⟩;
+  calc
+    t₁ = ⟨t₁.1, t₁.maximal, t₁.consistent⟩ := by rfl;
+    _  = ⟨t₂.1, t₂.maximal, t₂.consistent⟩ := by simp [e];
+    _  = t₂                                  := by rfl;
+
+lemma equality_of₂ (e₂ : t₁.1.2 = t₂.1.2) : t₁ = t₂ := equality_of₁ $ maximal_duality.mpr e₂
+
+
+lemma intro_equality {h₁ : ∀ {φ}, φ ∈ t₁.1.1 → φ ∈ t₂.1.1} {h₂ : ∀ {φ}, φ ∈ t₁.1.2 → φ ∈ t₂.1.2} : t₁ = t₂ := by
+  apply equality_of₁;
+  apply Set.eq_of_subset_of_subset;
+  . intro φ hφ;
+    exact h₁ hφ;
+  . intro φ;
+    contrapose;
+    intro hφ;
+    apply iff_not_mem₁_mem₂.mpr;
+    exact h₂ $ iff_not_mem₁_mem₂.mp hφ;
+
+section
+
+variable [DecidableEq α] [Encodable α]
+
+lemma iff_provable_include₁ : T *⊢[𝓢]! φ ↔ ∀ t : MaximalConsistentTableau 𝓢, (T ⊆ t.1.1) → φ ∈ t.1.1 := by
+  constructor;
+  . intro h t hT;
+    by_contra hφ;
+    replace hφ := iff_not_mem₁_mem₂.mp hφ;
+    obtain ⟨Γ, hΓ₁, hΓ₂⟩ := Context.provable_iff.mp h;
+    have := t.consistent (Γ := Γ) (Δ := [φ]) ?_ ?_;
+    contradiction;
+    . tauto_set;
+    . simpa;
+  . intro h;
+    by_contra hC;
+    obtain ⟨t, ht⟩ := lindenbaum (𝓢 := 𝓢) (t₀ := ⟨T, {φ}⟩) $ by
+      intro Γ Δ hΓ hΔ;
+      replace hΔ := by simpa using hΔ;
+      replace hC := Context.provable_iff.not.mp hC;
+      push_neg at hC;
+      have := hC Γ (by aesop);
+      suffices 𝓢 ⊬ ⋀Γ ➝ φ by
+        by_contra hC;
+        have : 𝓢 ⊢! ⋀Γ ➝ φ := imp_trans''! hC $ disj_allsame! $ by simpa
+        contradiction;
+      exact this;
+    have := iff_not_mem₂_mem₁.mpr $ h t ht.1;
+    have := ht.2;
+    tauto_set;
+
+lemma iff_provable_mem₁ : 𝓢 ⊢! φ ↔ ∀ t : MaximalConsistentTableau 𝓢, φ ∈ t.1.1 := by
+  constructor;
+  . intro h t;
+    apply iff_provable_include₁ (T := ∅) |>.mp;
+    . exact Context.of! h;
+    . simp;
+  . intro h;
+    exact Context.emptyPrf! $ iff_provable_include₁.mpr $ by tauto;
+
+end
+
+
+section Saturated
+
+variable [DecidableEq α] [Encodable α]
+
+omit [Encodable α] in
+lemma mdp_mem₁ (hφψ : φ ➝ ψ ∈ t.1.1) (hφ : φ ∈ t.1.1) : ψ ∈ t.1.1 := by
+  apply iff_not_mem₂_mem₁.mp;
+  by_contra hq₂;
+  have : 𝓢 ⊬ ⋀[φ, φ ➝ ψ] ➝ ⋁[ψ] := t.consistent (Γ := [φ, φ ➝ ψ]) (Δ := [ψ]) (by simp_all) (by simp_all);
+  have : 𝓢 ⊢! ⋀[φ, φ ➝ ψ] ➝ ⋁[ψ] := mdp_in!
+  contradiction;
+
+lemma mdp_mem₁_provable (hφψ : 𝓢 ⊢! φ ➝ ψ) (hφ : φ ∈ t.1.1) : ψ ∈ t.1.1 := mdp_mem₁ (iff_provable_mem₁.mp hφψ t) hφ
+
+lemma mdp_mem₂_provable (hφψ : 𝓢 ⊢! φ ➝ ψ) : ψ ∈ t.1.2 → φ ∈ t.1.2 := by
+  contrapose;
+  intro hφ;
+  apply iff_not_mem₂_mem₁.mpr;
+  apply mdp_mem₁_provable hφψ;
+  apply iff_not_mem₂_mem₁.mp hφ;
+
+
+@[simp] lemma mem₁_verum : ⊤ ∈ t.1.1 := iff_provable_mem₁.mp verum! t
+
+@[simp] lemma not_mem₂_verum : ⊤ ∉ t.1.2 := iff_not_mem₂_mem₁.mpr mem₁_verum
+
+
+omit [Encodable α] [DecidableEq α] in
+@[simp] lemma not_mem₁_falsum : ⊥ ∉ t.1.1 := disjoint.no_bot
+
+omit [Encodable α] [DecidableEq α] in
+@[simp] lemma mem₂_falsum : ⊥ ∈ t.1.2 := iff_not_mem₁_mem₂.mp not_mem₁_falsum
+
+
+private lemma of_mem₁_and : φ ⋏ ψ ∈ t.1.1 → (φ ∈ t.1.1 ∧ ψ ∈ t.1.1) := by
+  intro h;
+  constructor <;> exact mdp_mem₁_provable (by simp) h;
+
+private lemma of_mem₂_and : φ ⋏ ψ ∈ t.1.2 → (φ ∈ t.1.2 ∨ ψ ∈ t.1.2) := by
+  contrapose;
+  intro hφψ;
+  apply iff_not_mem₂_mem₁.mpr;
+  push_neg at hφψ;
+  have hφ := iff_not_mem₂_mem₁.mp hφψ.1;
+  have hψ := iff_not_mem₂_mem₁.mp hφψ.2;
+  exact mdp_mem₁ (mdp_mem₁_provable and₃! hφ) hψ;
+
+lemma iff_mem₁_and : φ ⋏ ψ ∈ t.1.1 ↔ (φ ∈ t.1.1 ∧ ψ ∈ t.1.1) := by
+  constructor;
+  . apply of_mem₁_and;
+  . contrapose;
+    push_neg;
+    intro hφψ hφ;
+    rcases of_mem₂_and $ iff_not_mem₁_mem₂.mp hφψ with (hφ | hψ);
+    . have := iff_not_mem₁_mem₂.mpr hφ; contradiction;
+    . exact iff_not_mem₁_mem₂.mpr hψ;
+
+lemma iff_mem₂_and : φ ⋏ ψ ∈ t.1.2 ↔ (φ ∈ t.1.2 ∨ ψ ∈ t.1.2) := by
+  constructor;
+  . apply of_mem₂_and;
+  . contrapose;
+    push_neg;
+    intro hφψ;
+    rcases of_mem₁_and $ iff_not_mem₂_mem₁.mp hφψ with ⟨hφ, hψ⟩;
+    constructor <;> { apply iff_not_mem₂_mem₁.mpr; assumption; };
+
+lemma iff_mem₁_conj {Γ : List _} : ⋀Γ ∈ t.1.1 ↔ (∀ φ ∈ Γ, φ ∈ t.1.1) := by
+  induction Γ using List.induction_with_singleton with
+  | hcons φ Γ hΓ ih =>
+    rw [List.conj₂_cons_nonempty hΓ]
+    constructor;
+    . intro h;
+      rcases iff_mem₁_and.mp h with ⟨hφ, hΓ⟩;
+      rintro ψ (hψ | hψ);
+      . assumption;
+      . apply ih.mp hΓ ψ;
+        assumption;
+    . intro h;
+      apply iff_mem₁_and.mpr;
+      constructor;
+      . apply h; tauto;
+      . apply ih.mpr;
+        intro ψ hψ;
+        apply h;
+        tauto;
+  | _ => simp;
+
+lemma iff_mem₂_conj {Γ : List _} : ⋀Γ ∈ t.1.2 ↔ (∃ φ ∈ Γ, φ ∈ t.1.2) := by
+  induction Γ using List.induction_with_singleton with
+  | hcons φ Γ hΓ ih =>
+    rw [List.conj₂_cons_nonempty hΓ];
+    constructor;
+    . intro h;
+      rcases iff_mem₂_and.mp h with (hφ | hΓ);
+      . exact ⟨φ, by tauto, hφ⟩;
+      . obtain ⟨ψ, hψ₁, hψ₂⟩ := ih.mp hΓ;
+        exact ⟨ψ, by tauto, hψ₂⟩;
+    . rintro ⟨ψ, (hψ₁ | hψ₁), hψ₂⟩;
+      . apply iff_mem₂_and.mpr;
+        left;
+        assumption;
+      . apply iff_mem₂_and.mpr;
+        right;
+        apply ih.mpr;
+        exact ⟨ψ, by simpa, hψ₂⟩;
+  | _ => simp;
+
+
+omit [DecidableEq α] [Encodable α] in
+private lemma of_mem₁_or : φ ⋎ ψ ∈ t.1.1 → (φ ∈ t.1.1 ∨ ψ ∈ t.1.1) := by
+  intro h;
+  by_contra hC;
+  push_neg at hC;
+  have : φ ∈ t.1.2 := iff_not_mem₁_mem₂.mp hC.1;
+  have : ψ ∈ t.1.2 := iff_not_mem₁_mem₂.mp hC.2;
+  have : 𝓢 ⊢! ⋀[φ ⋎ ψ] ➝ ⋁[φ, ψ] := by simp;
+  have : 𝓢 ⊬ ⋀[φ ⋎ ψ] ➝ ⋁[φ, ψ] := t.consistent (by simp_all) (by simp_all);
+  contradiction;
+
+private lemma of_mem₂_or : φ ⋎ ψ ∈ t.1.2 → (φ ∈ t.1.2 ∧ ψ ∈ t.1.2) := by
+  contrapose;
+  suffices (φ ∉ t.1.2 ∨ ψ ∉ t.1.2) → φ ⋎ ψ ∉ t.1.2 by tauto;
+  rintro (hφ | hψ);
+  . apply iff_not_mem₂_mem₁.mpr;
+    exact mdp_mem₁_provable or₁! $ iff_not_mem₂_mem₁.mp hφ;
+  . apply iff_not_mem₂_mem₁.mpr;
+    exact mdp_mem₁_provable or₂! $ iff_not_mem₂_mem₁.mp hψ;
+
+lemma iff_mem₁_or : φ ⋎ ψ ∈ t.1.1 ↔ (φ ∈ t.1.1 ∨ ψ ∈ t.1.1) := by
+  constructor;
+  . apply of_mem₁_or;
+  . contrapose;
+    push_neg;
+    intro hφψ;
+    rcases of_mem₂_or $ iff_not_mem₁_mem₂.mp hφψ with ⟨hφ, hψ⟩;
+    constructor <;> { apply iff_not_mem₁_mem₂.mpr; assumption; };
+
+lemma iff_mem₂_or : φ ⋎ ψ ∈ t.1.2 ↔ (φ ∈ t.1.2 ∧ ψ ∈ t.1.2) := by
+  constructor;
+  . apply of_mem₂_or;
+  . contrapose;
+    push_neg;
+    intro hφψ hφ;
+    rcases of_mem₁_or $ iff_not_mem₂_mem₁.mp hφψ with (hφ | hψ);
+    . have := iff_not_mem₂_mem₁.mpr hφ; contradiction;
+    . exact iff_not_mem₂_mem₁.mpr hψ;
+
+lemma iff_mem₁_disj  {Γ : List _} : ⋁Γ ∈ t.1.1 ↔ (∃ φ ∈ Γ, φ ∈ t.1.1) := by
+  induction Γ using List.induction_with_singleton with
+  | hcons φ Γ hΓ ih =>
+    rw [List.disj₂_cons_nonempty hΓ];
+    constructor;
+    . intro h;
+      rcases iff_mem₁_or.mp h with (hφ | hΓ);
+      . exact ⟨φ, by tauto, hφ⟩;
+      . obtain ⟨ψ, hψ₁, hψ₂⟩ := ih.mp hΓ;
+        exact ⟨ψ, by tauto, hψ₂⟩;
+    . rintro ⟨ψ, (hψ₁ | hψ₁), hψ₂⟩;
+      . apply iff_mem₁_or.mpr;
+        left;
+        assumption;
+      . apply iff_mem₁_or.mpr;
+        right;
+        apply ih.mpr;
+        exact ⟨ψ, by simpa, hψ₂⟩;
+  | _ => simp;
+
+lemma iff_mem₂_disj {Γ : List _} : ⋁Γ ∈ t.1.2 ↔ (∀ φ ∈ Γ, φ ∈ t.1.2) := by
+  induction Γ using List.induction_with_singleton with
+  | hcons φ Γ hΓ ih =>
+    rw [List.disj₂_cons_nonempty hΓ];
+    constructor;
+    . intro h;
+      rcases iff_mem₂_or.mp h with ⟨hφ, hΓ⟩;
+      rintro ψ (hψ | hΓ);
+      . assumption;
+      . apply ih.mp hΓ;
+        assumption;
+    . intro h;
+      apply iff_mem₂_or.mpr;
+      constructor;
+      . apply h; tauto;
+      . apply ih.mpr;
+        intro ψ hψ;
+        apply h;
+        tauto;
+  | _ => simp;
+
+
+omit [Encodable α] in
+private lemma of_mem₁_imp : φ ➝ ψ ∈ t.1.1 → (φ ∈ t.1.2 ∨ ψ ∈ t.1.1) := by
+  intro h;
+  by_contra hC;
+  push_neg at hC;
+  exact hC.2 $ mdp_mem₁ h $ iff_not_mem₂_mem₁.mp hC.1
+
+private lemma of_mem₂_imp : φ ➝ ψ ∈ t.1.2 → (φ ∈ t.1.1 ∧ ψ ∈ t.1.2) := by
+  intro h;
+  by_contra hC;
+  replace hC := not_and_or.mp hC;
+  rcases hC with (hφ | hψ);
+  . have : φ ⋎ (φ ➝ ψ) ∈ t.1.1 := iff_provable_mem₁.mp (or_replace_right'! lem! efq_imply_not₁!) t;
+    rcases of_mem₁_or this with (_ | _);
+    . contradiction;
+    . have := iff_not_mem₁_mem₂.mpr h;
+      contradiction;
+  . have : ψ ➝ (φ ➝ ψ) ∈ t.1.1 := iff_provable_mem₁.mp imply₁! t;
+    have : φ ➝ ψ ∉ t.1.2 := iff_not_mem₂_mem₁.mpr $ mdp_mem₁ this (iff_not_mem₂_mem₁.mp hψ);
+    contradiction;
+
+lemma iff_mem₁_imp : φ ➝ ψ ∈ t.1.1 ↔ (φ ∈ t.1.2 ∨ ψ ∈ t.1.1) := by
+  constructor;
+  . apply of_mem₁_imp;
+  . contrapose;
+    push_neg;
+    intro hφψ;
+    rcases of_mem₂_imp $ iff_not_mem₁_mem₂.mp hφψ with ⟨hφ, hψ⟩;
+    constructor;
+    . exact iff_not_mem₂_mem₁.mpr hφ;
+    . exact iff_not_mem₁_mem₂.mpr hψ;
+
+lemma iff_mem₂_imp : φ ➝ ψ ∈ t.1.2 ↔ (φ ∈ t.1.1 ∧ ψ ∈ t.1.2) := by
+  constructor;
+  . apply of_mem₂_imp;
+  . contrapose;
+    push_neg;
+    intro hφψ hφ;
+    rcases of_mem₁_imp $ iff_not_mem₂_mem₁.mp hφψ with (hφ | hψ);
+    . have := iff_not_mem₁_mem₂.mpr hφ; contradiction;
+    . exact iff_not_mem₂_mem₁.mpr hψ;
+
+
+omit [Encodable α] in
+private lemma of_mem₁_neg : ∼φ ∈ t.1.1 → (φ ∈ t.1.2) := by
+  intro h;
+  rcases of_mem₁_imp h with (hφ | hb);
+  . assumption;
+  . exfalso;
+    exact not_mem₁_falsum hb;
+
+private lemma of_mem₂_neg : ∼φ ∈ t.1.2 → (φ ∈ t.1.1) := by
+  intro h;
+  rcases of_mem₂_imp h with ⟨hφ, hb⟩;
+  exact hφ;
+
+lemma iff_mem₁_neg : ∼φ ∈ t.1.1 ↔ φ ∈ t.1.2 := by
+  constructor;
+  . apply of_mem₁_neg;
+  . contrapose;
+    intro h;
+    exact iff_not_mem₂_mem₁.mpr $ of_mem₂_neg $ iff_not_mem₁_mem₂.mp h
+
+lemma iff_mem₂_neg : ∼φ ∈ t.1.2 ↔ φ ∈ t.1.1 := by
+  constructor;
+  . apply of_mem₂_neg;
+  . contrapose;
+    intro h;
+    exact iff_not_mem₁_mem₂.mpr $ of_mem₁_neg $ iff_not_mem₂_mem₁.mp h
+
+
+omit [Entailment.K 𝓢] [DecidableEq α] [Encodable α] in
+private lemma of_mem₁_multibox : (□^[n]φ ∈ t.1.1) → (∀ {t' : MaximalConsistentTableau 𝓢}, (□''⁻¹^[n]t.1.1 ⊆ t'.1.1) → (φ ∈ t'.1.1)) := by
+  intro h t' ht';
+  apply ht';
+  tauto;
+
+private lemma of_mem₂_multibox : (□^[n]φ ∈ t.1.2) → (∃ t' : MaximalConsistentTableau 𝓢, (□''⁻¹^[n]t.1.1 ⊆ t'.1.1) ∧ (φ ∈ t'.1.2)) := by
+  intro h;
+  obtain ⟨t', ht'⟩ := lindenbaum (𝓢 := 𝓢) (t₀ := ⟨□''⁻¹^[n]t.1.1, {φ}⟩) $ by
+    intro Γ Δ hΓ hΔ;
+    by_contra hC;
+    have h₁ : 𝓢 ⊢! ⋀□'^[n]Γ ➝ □^[n]⋀Γ := collect_multibox_conj!
+    have : 𝓢 ⊢! ⋀□'^[n]Γ ➝ □^[n]φ := imp_trans''! h₁ (imply_multibox_distribute'! $ imp_trans''! hC (disj_allsame! hΔ));
+    have : 𝓢 ⊬ ⋀□'^[n]Γ ➝ ⋁[□^[n]φ] := t.consistent (Γ := □'^[n]Γ) (Δ := [□^[n]φ]) ?_ ?_;
+    contradiction;
+    . rintro ψ hψ;
+      obtain ⟨ξ, hξ, rfl⟩ := List.exists_of_multibox hψ;
+      exact hΓ ξ hξ;
+    . simpa;
+  use t';
+  constructor;
+  . exact ht'.1;
+  . apply ht'.2;
+    tauto;
+
+lemma iff_mem₁_multibox : (□^[n]φ ∈ t.1.1) ↔ (∀ {t' : MaximalConsistentTableau 𝓢}, (□''⁻¹^[n]t.1.1 ⊆ t'.1.1) → (φ ∈ t'.1.1)) := by
+  constructor;
+  . apply of_mem₁_multibox;
+  . contrapose;
+    push_neg;
+    intro hφ;
+    obtain ⟨t', ht'₁, ht'₂⟩ := of_mem₂_multibox $ iff_not_mem₁_mem₂.mp hφ;
+    use t';
+    constructor;
+    . exact ht'₁;
+    . exact iff_not_mem₁_mem₂.mpr ht'₂;
+
+lemma iff_mem₁_box : (□φ ∈ t.1.1) ↔ (∀ {t' : MaximalConsistentTableau 𝓢}, (□''⁻¹t.1.1 ⊆ t'.1.1) → (φ ∈ t'.1.1)) := iff_mem₁_multibox (n := 1)
+
+lemma iff_mem₂_multibox : (□^[n]φ ∈ t.1.2) ↔ (∃ t' : MaximalConsistentTableau 𝓢, (□''⁻¹^[n]t.1.1 ⊆ t'.1.1) ∧ (φ ∈ t'.1.2)) := by
+  constructor;
+  . apply of_mem₂_multibox;
+  . contrapose;
+    push_neg;
+    intro hφ t' ht';
+    exact iff_not_mem₂_mem₁.mpr $ of_mem₁_multibox (iff_not_mem₂_mem₁.mp hφ) ht';
+
+lemma iff_mem₂_box : (□φ ∈ t.1.2) ↔ (∃ t' : MaximalConsistentTableau 𝓢, (□''⁻¹t.1.1 ⊆ t'.1.1) ∧ (φ ∈ t'.1.2)) := iff_mem₂_multibox (n := 1)
+
+
+
+end Saturated
+
+end MaximalConsistentTableau
+
+end LO.Modal
